modify rules and fix some holes

proof/iu_system/decl/def_extra.v
@@ -51,10 +51,10 @@ Inductive dwf_typ_s : denv -> dtyp -> Prop :=    (* defn dwf_typ_s *)
      dwf_typ_s E T1 ->
      dwf_typ_s E T2 ->
      dwf_typ_s E (dtyp_arrow T1 T2)
- | dwftyps_all : forall (L:vars) (E:denv) (T:dtyp),
-     ( forall SX , SX \notin L -> ds_in_s SX  (open_dtyp_wrt_dtyp  T   (dtyp_svar SX) ) ) ->
-     ( forall SX , SX \notin L -> dwf_typ_s  ( SX ~ dbind_stvar_empty  ++  E )   (open_dtyp_wrt_dtyp  T   (dtyp_svar SX) ) ) ->
-     dwf_typ_s E (dtyp_all T)
+ | dwftyps_all : forall (L:vars) (E:denv) (T1:dtyp),
+     ( forall SX , SX \notin L -> ds_in_s SX  (open_dtyp_wrt_dtyp  T1   (dtyp_svar SX) ) ) ->
+     ( forall SX , SX \notin L -> dwf_typ_s  ( SX ~ dbind_stvar_empty  ++  E )   (open_dtyp_wrt_dtyp  T1   (dtyp_svar SX) ) ) ->
+     dwf_typ_s E (dtyp_all T1)
  | dwftyps_union : forall (E:denv) (T1 T2:dtyp),
      dwf_typ_s E T1 ->
      dwf_typ_s E T2 ->
@@ -64,154 +64,154 @@ Inductive dwf_typ_s : denv -> dtyp -> Prop :=    (* defn dwf_typ_s *)
      dwf_typ_s E T2 ->
      dwf_typ_s E (dtyp_intersection T1 T2).
 
-Inductive dsub : denv -> dtyp -> dtyp -> Prop :=    (* defn dsub *)
- | dsub_top : forall (E:denv) (S:dtyp),
-     dwf_typ E S ->
-     dsub E S dtyp_top
- | dsub_bot : forall (E:denv) (T:dtyp),
-     dwf_typ E T ->
-     dsub E dtyp_bot T
- | dsub_unit : forall (E:denv),
-     dsub E dtyp_unit dtyp_unit
- | dsub_tvar : forall (E:denv) (X:typvar),
+Inductive d_sub : denv -> dtyp -> dtyp -> Prop :=    (* defn d_sub *)
+ | d_sub_top : forall (E:denv) (S1:dtyp),
+     dwf_typ E S1 ->
+     d_sub E S1 dtyp_top
+ | d_sub_bot : forall (E:denv) (T1:dtyp),
+     dwf_typ E T1 ->
+     d_sub E dtyp_bot T1
+ | d_sub_unit : forall (E:denv),
+     d_sub E dtyp_unit dtyp_unit
+ | d_sub_tvar : forall (E:denv) (X:typvar),
      dwf_typ E (dtyp_var_f X) ->
-     dsub E (dtyp_var_f X) (dtyp_var_f X)
- | dsub_stvar : forall (E:denv) (SX:stypvar),
+     d_sub E (dtyp_var_f X) (dtyp_var_f X)
+ | d_sub_stvar : forall (E:denv) (SX:stypvar),
      dwf_typ E (dtyp_svar SX) ->
-     dsub E (dtyp_svar SX) (dtyp_svar SX)
- | dsub_arrow : forall (E:denv) (S1 S2 T1 T2:dtyp),
-     dsub E T1 S1 ->
-     dsub E S2 T2 ->
-     dsub E (dtyp_arrow S1 S2) (dtyp_arrow T1 T2)
- | dsub_all : forall (L:vars) (E:denv) (S T:dtyp),
-     ( forall SX , SX \notin L -> ds_in_s SX  (open_dtyp_wrt_dtyp  S   (dtyp_svar SX) ) ) ->
-     ( forall SX , SX \notin L -> ds_in_s SX  (open_dtyp_wrt_dtyp  T   (dtyp_svar SX) ) ) ->
-     ( forall SX , SX \notin L -> dsub  ( SX ~ dbind_stvar_empty  ++  E )   (open_dtyp_wrt_dtyp  S   (dtyp_svar SX) )   (open_dtyp_wrt_dtyp  T   (dtyp_svar SX) ) ) ->
-     dsub E (dtyp_all S) (dtyp_all T)
- | dsub_alll : forall (L:vars) (E:denv) (S T1 T2:dtyp),
+     d_sub E (dtyp_svar SX) (dtyp_svar SX)
+ | d_sub_arrow : forall (E:denv) (S1 S2 T1 T2:dtyp),
+     d_sub E T1 S1 ->
+     d_sub E S2 T2 ->
+     d_sub E (dtyp_arrow S1 S2) (dtyp_arrow T1 T2)
+ | d_sub_all : forall (L:vars) (E:denv) (S1 T1:dtyp),
+     ( forall SX , SX \notin L -> ds_in_s SX  (open_dtyp_wrt_dtyp  S1   (dtyp_svar SX) ) ) ->
+     ( forall SX , SX \notin L -> ds_in_s SX  (open_dtyp_wrt_dtyp  T1   (dtyp_svar SX) ) ) ->
+     ( forall SX , SX \notin L -> d_sub  ( SX ~ dbind_stvar_empty  ++  E )   (open_dtyp_wrt_dtyp  S1   (dtyp_svar SX) )   (open_dtyp_wrt_dtyp  T1   (dtyp_svar SX) ) ) ->
+     d_sub E (dtyp_all S1) (dtyp_all T1)
+ | d_sub_alll : forall (L:vars) (E:denv) (S1 T1 T2:dtyp),
      dneq_all T1 ->
-     dneq_intersection T1 ->
-     dneq_union T1 -> 
-     ( forall X , X \notin L -> ds_in X  (open_dtyp_wrt_dtyp  S   (dtyp_var_f X) ) ) ->
+     (* dneq_intersection T1 -> *)
+     (* dneq_union T1 ->  *)
+     ( forall X , X \notin L -> ds_in X  (open_dtyp_wrt_dtyp  S1   (dtyp_var_f X) ) ) ->
      dwf_typ E T2 ->
      dmono_typ T2 ->
-     dsub E  (open_dtyp_wrt_dtyp  S   T2 )  T1 ->
-     dsub E (dtyp_all S) T1
- | dsub_intersection1 : forall (E:denv) (S T1 T2:dtyp),
-     dsub E S T1 ->
-     dsub E S T2 ->
-     dsub E S (dtyp_intersection T1 T2)
- | dsub_intersection2 : forall (E:denv) (S1 S2 T:dtyp),
-     dsub E S1 T ->
+     d_sub E  (open_dtyp_wrt_dtyp  S1   T2 )  T1 ->
+     d_sub E (dtyp_all S1) T1
+ | d_sub_intersection1 : forall (E:denv) (S1 T1 T2:dtyp),
+     d_sub E S1 T1 ->
+     d_sub E S1 T2 ->
+     d_sub E S1 (dtyp_intersection T1 T2)
+ | d_sub_intersection2 : forall (E:denv) (S1 S2 T1:dtyp),
+     d_sub E S1 T1 ->
      dwf_typ E S2 ->
-     dsub E (dtyp_intersection S1 S2) T
- | dsub_intersection3 : forall (E:denv) (S1 S2 T:dtyp),
-     dsub E S2 T ->
+     d_sub E (dtyp_intersection S1 S2) T1
+ | d_sub_intersection3 : forall (E:denv) (S1 S2 T1:dtyp),
+     d_sub E S2 T1 ->
      dwf_typ E S1 ->
-     dsub E (dtyp_intersection S1 S2) T
- | dsub_union1 : forall (E:denv) (S T1 T2:dtyp),
-     dsub E S T1 ->
+     d_sub E (dtyp_intersection S1 S2) T1
+ | d_sub_union1 : forall (E:denv) (S1 T1 T2:dtyp),
+     d_sub E S1 T1 ->
      dwf_typ E T2 ->
-     dsub E S (dtyp_union T1 T2)
- | dsub_union2 : forall (E:denv) (S T1 T2:dtyp),
-     dsub E S T2 ->
+     d_sub E S1 (dtyp_union T1 T2)
+ | d_sub_union2 : forall (E:denv) (S1 T1 T2:dtyp),
+     d_sub E S1 T2 ->
      dwf_typ E T1 ->
-     dsub E S (dtyp_union T1 T2)
- | dsub_union3 : forall (E:denv) (S1 S2 T:dtyp),
-     dsub E S1 T ->
-     dsub E S2 T ->
-     dsub E (dtyp_union S1 S2) T.
+     d_sub E S1 (dtyp_union T1 T2)
+ | d_sub_union3 : forall (E:denv) (S1 S2 T1:dtyp),
+     d_sub E S1 T1 ->
+     d_sub E S2 T1 ->
+     d_sub E (dtyp_union S1 S2) T1.
 
-Inductive dtyping_mode :=
-    | dtypingmode_inf 
-    | dtypingmode_chk
-    | dtypingmode_infapp (t : dtyp).
+Inductive d_typing_mode :=
+    | d_typingmode_inf 
+    | d_typingmode_chk
+    | d_typingmode_infapp (T1 : dtyp).
 
-Definition dsubst_tv_in_dtypingmode (T1:dtyp) (X:typvar) (m:dtyping_mode):=
+Definition d_subst_tv_in_typingmode (T1:dtyp) (X:typvar) (m:d_typing_mode):=
     match m with 
-    | dtypingmode_chk => dtypingmode_chk
-    | dtypingmode_inf => dtypingmode_inf
-    | dtypingmode_infapp T2 => dtypingmode_infapp (dsubst_tv_in_dtyp T1 X T2)
+    | d_typingmode_chk => d_typingmode_chk
+    | d_typingmode_inf => d_typingmode_inf
+    | d_typingmode_infapp T2 => d_typingmode_infapp (d_subst_tv_in_dtyp T1 X T2)
     end.
 
-Inductive dtyping : denv -> dexp -> dtyping_mode -> dtyp -> Prop :=
-| dtyping_infvar : forall (E:denv) (x:expvar) (T:dtyp),
+Inductive d_typing : denv -> dexp -> d_typing_mode -> dtyp -> Prop :=
+| d_typing_infvar : forall (E:denv) (x:expvar) (T1:dtyp),
     dwf_env E ->
-    binds ( x )  ( (dbind_typ T) ) ( E )  ->
-    dtyping E (dexp_var_f x) dtypingmode_inf T
-| dtyping_infanno : forall (E:denv) (e:dexp) (T:dtyp),
-    dwf_typ E T ->
-    dtyping E e dtypingmode_chk T ->
-    dtyping E  ( (dexp_anno e T) )  dtypingmode_inf T
-| dtypinginf_unit : forall (E:denv),
-    dwf_env E ->
-    dtyping E dexp_unit dtypingmode_inf dtyp_unit
-| dtyping_infapp : forall (E:denv) (e1 e2:dexp) (T1 T2:dtyp),
-    dtyping E e1 dtypingmode_inf T2 ->
-    dtyping E e2 (dtypingmode_infapp T2) T1 ->
-    dtyping E  ( (dexp_app e1 e2) ) dtypingmode_inf T1
-| dtyping_inftabs : forall (L:vars) (E:denv) (e:dexp) (T:dtyp),
-dwf_typ E (dtyp_all T) ->
-    ( forall X , X \notin  L  -> dtyping  ( X ~ dbind_tvar_empty  ++  E ) (dexp_anno  ( open_dexp_wrt_dtyp e (dtyp_var_f X) )  ( open_dtyp_wrt_dtyp T (dtyp_var_f X) ) ) dtypingmode_chk ( open_dtyp_wrt_dtyp T (dtyp_var_f X) )  )  ->
-    dtyping E (dexp_tabs (dbody_anno e T)) dtypingmode_inf (dtyp_all T)
-| dtyping_inftappbot : forall (E:denv) (e:dexp) (T:dtyp),
-    dwf_typ E T ->
-    dtyping E e dtypingmode_inf dtyp_bot ->
-    dtyping E (dexp_tapp e T) dtypingmode_inf dtyp_bot
-| dtyping_inftappall : forall (E:denv) (e1:dexp) (T2 T1:dtyp),
-    dwf_typ E T2 ->
-    dtyping E e1 dtypingmode_inf (dtyp_all T1) ->
-    dtyping E (dexp_tapp e1 T2) dtypingmode_inf (open_dtyp_wrt_dtyp  T1 T2 ) 
-| dtyping_chkabstop : forall (L:vars) (E:denv) (e:dexp),
-    ( forall x , x \notin  L  -> dtyping  ( x ~ (dbind_typ dtyp_bot)  ++  E )   ( open_dexp_wrt_dexp e (dexp_var_f x) ) dtypingmode_chk dtyp_top )  ->
-    dtyping E (dexp_abs e) dtypingmode_chk dtyp_top
-| dtyping_chkabs : forall (L:vars) (E:denv) (e:dexp) (T1 T2:dtyp),
+    binds ( x )  ( (dbind_typ T1) ) ( E )  ->
+    d_typing E (dexp_var_f x) d_typingmode_inf T1
+| d_typing_infanno : forall (E:denv) (e:dexp) (T1:dtyp),
     dwf_typ E T1 ->
-    ( forall x , x \notin  L  -> dtyping  ( x ~ (dbind_typ T1)  ++  E )  ( open_dexp_wrt_dexp e (dexp_var_f x) ) dtypingmode_chk T2 )  ->
-    dtyping E (dexp_abs e) dtypingmode_chk (dtyp_arrow T1 T2)
-| dtyping_chkall : forall (L:vars) (E:denv) (e:dexp) (T:dtyp),
-    dwf_typ E (dtyp_all T) ->
-    ( forall X , X \notin  L  -> dtyping  ( X ~ dbind_tvar_empty  ++  E )  e  dtypingmode_chk ( open_dtyp_wrt_dtyp T (dtyp_var_f X) )  )  ->
-    dtyping E e dtypingmode_chk (dtyp_all T)
-| dtyping_chksub : forall (E:denv) (e:dexp) (T S:dtyp),
-    dtyping E e dtypingmode_inf S ->
-    dsub E S T ->
-    dtyping E e dtypingmode_chk T
-| dtyping_chkintersection : forall (E:denv) (e:dexp) (S T:dtyp),
-    dtyping E e dtypingmode_chk S ->
-    dtyping E e dtypingmode_chk T ->
-    dtyping E e dtypingmode_chk (dtyp_intersection S T)
-| dtyping_chkunion1 : forall (E:denv) (e:dexp) (S T:dtyp),
-    dtyping E e dtypingmode_chk S ->
-    dwf_typ E T ->
-    dtyping E e dtypingmode_chk (dtyp_union S T)
-| dtyping_chkunion2 : forall (E:denv) (e:dexp) (S T:dtyp),
-    dtyping E e dtypingmode_chk T ->
-    dwf_typ E S ->
-    dtyping E e dtypingmode_chk (dtyp_union S T)
-| dtyping_infapparrow : forall (E:denv) (T1 T2:dtyp) (e:dexp),
+    d_typing E e d_typingmode_chk T1 ->
+    d_typing E  ( (dexp_anno e T1) )  d_typingmode_inf T1
+| d_typinginf_unit : forall (E:denv),
+    dwf_env E ->
+    d_typing E dexp_unit d_typingmode_inf dtyp_unit
+| d_typing_infapp : forall (E:denv) (e1 e2:dexp) (T1 T2:dtyp),
+    d_typing E e1 d_typingmode_inf T2 ->
+    d_typing E e2 (d_typingmode_infapp T2) T1 ->
+    d_typing E  ( (dexp_app e1 e2) ) d_typingmode_inf T1
+| d_typing_inftabs : forall (L:vars) (E:denv) (e:dexp) (T1:dtyp),
+dwf_typ E (dtyp_all T1) ->
+    ( forall X , X \notin  L  -> d_typing  ( X ~ dbind_tvar_empty  ++  E ) (dexp_anno  ( open_dexp_wrt_dtyp e (dtyp_var_f X) )  ( open_dtyp_wrt_dtyp T1 (dtyp_var_f X) ) ) d_typingmode_chk ( open_dtyp_wrt_dtyp T1 (dtyp_var_f X) )  )  ->
+    d_typing E (dexp_tabs (dbody_anno e T1)) d_typingmode_inf (dtyp_all T1)
+| d_typing_inftappbot : forall (E:denv) (e:dexp) (T1:dtyp),
+    dwf_typ E T1 ->
+    d_typing E e d_typingmode_inf dtyp_bot ->
+    d_typing E (dexp_tapp e T1) d_typingmode_inf dtyp_bot
+| d_typing_inftappall : forall (E:denv) (e1:dexp) (T2 T1:dtyp),
     dwf_typ E T2 ->
-    dtyping E e dtypingmode_chk T1 ->
-    dtyping E e ( dtypingmode_infapp ( (dtyp_arrow T1 T2) ) ) T2
-| dtyping_infappall : forall (E:denv) (T1:dtyp) (e:dexp) (T2 T3:dtyp),
+    d_typing E e1 d_typingmode_inf (dtyp_all T1) ->
+    d_typing E (dexp_tapp e1 T2) d_typingmode_inf (open_dtyp_wrt_dtyp  T1 T2 ) 
+| d_typing_chkabstop : forall (L:vars) (E:denv) (e:dexp),
+    ( forall x , x \notin  L  -> d_typing  ( x ~ (dbind_typ dtyp_bot)  ++  E )   ( open_dexp_wrt_dexp e (dexp_var_f x) ) d_typingmode_chk dtyp_top )  ->
+    d_typing E (dexp_abs e) d_typingmode_chk dtyp_top
+| d_typing_chkabs : forall (L:vars) (E:denv) (e:dexp) (T1 T2:dtyp),
+    dwf_typ E T1 ->
+    ( forall x , x \notin  L  -> d_typing  ( x ~ (dbind_typ T1)  ++  E )  ( open_dexp_wrt_dexp e (dexp_var_f x) ) d_typingmode_chk T2 )  ->
+    d_typing E (dexp_abs e) d_typingmode_chk (dtyp_arrow T1 T2)
+| d_typing_chkall : forall (L:vars) (E:denv) (e:dexp) (T1:dtyp),
+    dwf_typ E (dtyp_all T1) ->
+    ( forall X , X \notin  L  -> d_typing  ( X ~ dbind_tvar_empty  ++  E )  e  d_typingmode_chk ( open_dtyp_wrt_dtyp T1 (dtyp_var_f X) )  )  ->
+    d_typing E e d_typingmode_chk (dtyp_all T1)
+| d_typing_chksub : forall (E:denv) (e:dexp) (T1 S1:dtyp),
+    d_typing E e d_typingmode_inf S1 ->
+    d_sub E S1 T1 ->
+    d_typing E e d_typingmode_chk T1
+| d_typing_chkintersection : forall (E:denv) (e:dexp) (S1 T1:dtyp),
+    d_typing E e d_typingmode_chk S1 ->
+    d_typing E e d_typingmode_chk T1 ->
+    d_typing E e d_typingmode_chk (dtyp_intersection S1 T1)
+| d_typing_chkunion1 : forall (E:denv) (e:dexp) (S1 T1:dtyp),
+    d_typing E e d_typingmode_chk S1 ->
+    dwf_typ E T1 ->
+    d_typing E e d_typingmode_chk (dtyp_union S1 T1)
+| d_typing_chkunion2 : forall (E:denv) (e:dexp) (S1 T1:dtyp),
+    d_typing E e d_typingmode_chk T1 ->
+    dwf_typ E S1 ->
+    d_typing E e d_typingmode_chk (dtyp_union S1 T1)
+| d_typing_infapparrow : forall (E:denv) (T1 T2:dtyp) (e:dexp),
+    dwf_typ E T2 ->
+    d_typing E e d_typingmode_chk T1 ->
+    d_typing E e ( d_typingmode_infapp ( (dtyp_arrow T1 T2) ) ) T2
+| d_typing_infappall : forall (E:denv) (T1:dtyp) (e:dexp) (T2 T3:dtyp),
     dmono_typ T3 ->
     dwf_typ E T3 ->
     dwf_typ E (dtyp_all T1) ->
-    dtyping E e ( dtypingmode_infapp (open_dtyp_wrt_dtyp  T1   T3 ) )T2 ->
-    dtyping E e ( dtypingmode_infapp ( (dtyp_all T1) ) ) T2
-| dtyping_infappbot : forall (E:denv) (e:dexp),
-    dtyping E e dtypingmode_chk dtyp_top ->
-    dtyping E e ( dtypingmode_infapp dtyp_bot ) dtyp_bot
-| dtyping_infappintersection1 : forall (E:denv) (e:dexp) (S1 S2 T:dtyp),
-    dtyping E e ( dtypingmode_infapp S1 ) T ->
-    dtyping E e ( dtypingmode_infapp (dtyp_intersection S1 S2) ) T
-| dtyping_infappintersection2 : forall (E:denv) (e:dexp) (S1 S2 T:dtyp),
-    dtyping E e ( dtypingmode_infapp S2 ) T ->
-    dtyping E e ( dtypingmode_infapp (dtyp_intersection S1 S2) ) T 
-| dtyping_infappunion : forall (E:denv) (e:dexp) (S1 S2 T:dtyp),
-    dtyping E e ( dtypingmode_infapp S1 ) T ->
-    dtyping E e ( dtypingmode_infapp S2 ) T ->
-    dtyping E e ( dtypingmode_infapp (dtyp_union S1 S2) ) T
+    d_typing E e ( d_typingmode_infapp (open_dtyp_wrt_dtyp  T1   T3 ) )T2 ->
+    d_typing E e ( d_typingmode_infapp ( (dtyp_all T1) ) ) T2
+| d_typing_infappbot : forall (E:denv) (e:dexp),
+    d_typing E e d_typingmode_chk dtyp_top ->
+    d_typing E e ( d_typingmode_infapp dtyp_bot ) dtyp_bot
+| d_typing_infappintersection1 : forall (E:denv) (e:dexp) (S1 S2 T1:dtyp),
+    d_typing E e ( d_typingmode_infapp S1 ) T1 ->
+    d_typing E e ( d_typingmode_infapp (dtyp_intersection S1 S2) ) T1
+| d_typing_infappintersection2 : forall (E:denv) (e:dexp) (S1 S2 T1:dtyp),
+    d_typing E e ( d_typingmode_infapp S2 ) T1 ->
+    d_typing E e ( d_typingmode_infapp (dtyp_intersection S1 S2) ) T1 
+| d_typing_infappunion : forall (E:denv) (e:dexp) (S1 S2 T1:dtyp),
+    d_typing E e ( d_typingmode_infapp S1 ) T1 ->
+    d_typing E e ( d_typingmode_infapp S2 ) T1 ->
+    d_typing E e ( d_typingmode_infapp (dtyp_union S1 S2) ) T1
     .
 
 
