proof/iu_system/decl/prop_basic.v
@@ -4,14 +4,361 @@ Require Import Lia.
 Require Import Metalib.Metatheory.
 
 Require Import decl.notations.
-Require Import decl.prop_ln_extra.
 Require Import ln_utils.
-
 
 Hint Constructors dwf_typ: core.
 Hint Constructors dwf_env: core.
 Hint Constructors dwf_typ_s: core.
 
+
+Lemma subst_same_tvar_eq : forall T X,
+  T = {`ᵈ X /ᵈ X} T.
+Proof.
+  intros.
+  induction T; auto; simpl.
+  - destruct (X0==X); subst; auto. 
+  - simpl. rewrite <- IHT1. rewrite <- IHT2. auto.
+  - simpl. rewrite <- IHT. auto.
+  - simpl. rewrite <- IHT1. rewrite <- IHT2. auto.
+  - simpl. rewrite <- IHT1. rewrite <- IHT2. auto.
+Qed.
+
+Lemma fstv_in_dtyp_open_dtyp_wrt_dtyp_rec_upper_mutual :
+(forall T1 T2 n1,
+  fstv_in_dtyp (open_dtyp_wrt_dtyp_rec n1 T2 T1) [<=] fstv_in_dtyp T2 `union` fstv_in_dtyp T1).
+Proof.
+  apply_mutual_ind dtyp_mutind;
+  default_simp; try fsetdec.
+  - rewrite IHdtyp1; rewrite IHdtyp2. fsetdec.
+  - rewrite IHdtyp1; rewrite IHdtyp2. fsetdec.
+  - rewrite IHdtyp1; rewrite IHdtyp2. fsetdec.
+Qed.
+
+Lemma fstv_in_dtyp_open_dtyp_wrt_dtyp_rec_upper : forall T1 T2 n1,
+  fstv_in_dtyp (open_dtyp_wrt_dtyp_rec n1 T2 T1) [<=] fstv_in_dtyp T2 `union` fstv_in_dtyp T1.
+Proof.
+  pose proof fstv_in_dtyp_open_dtyp_wrt_dtyp_rec_upper_mutual as H; intuition eauto.
+Qed.
+
+Lemma fstv_in_dtyp_open_dtyp_wrt_dtyp_upper : forall T1 T2,
+  fstv_in_dtyp (open_dtyp_wrt_dtyp T1 T2) [<=] fstv_in_dtyp T2 `union` fstv_in_dtyp T1.
+Proof.
+  intros.
+  unfold open_dtyp_wrt_dtyp.
+  apply fstv_in_dtyp_open_dtyp_wrt_dtyp_rec_upper.
+Qed.
+
+Lemma dtyp_subst_open_comm : forall X T1 T2 T3,
+  lc_dtyp T2 -> 
+  X `notin` ftv_in_dtyp T3 -> 
+  ({T2 /ᵈ X} T1) ^^ᵈ T3 = {T2 /ᵈ X} T1 ^^ᵈ T3.
+Proof.
+  intros.
+  rewrite d_subst_tv_in_dtyp_open_dtyp_wrt_dtyp; auto.
+  rewrite (d_subst_tv_in_dtyp_fresh_eq T3); auto.
+Qed.
+
+
+Lemma dtyp_open_r_close_l : forall T1 T2 X
+  , X `notin` ftv_in_dtyp T2
+  -> T1 = open_dtyp_wrt_dtyp T2 `ᵈ X -> close_dtyp_wrt_dtyp X T1 = T2.
+Proof.
+  intros * Fr H.
+  assert (close_dtyp_wrt_dtyp X T1 = close_dtyp_wrt_dtyp X (open_dtyp_wrt_dtyp T2 `ᵈ X)) by now rewrite H.
+  now rewrite close_dtyp_wrt_dtyp_open_dtyp_wrt_dtyp in H0.
+Qed.
+
+
+Lemma close_dtyp_notin_rec : forall X e n,
+    X `notin` ftv_in_dtyp (close_dtyp_wrt_dtyp_rec n X e).
+Proof.
+  intros until e.
+  induction e; simpl; intros; auto.
+  - destruct (lt_dec n n0); auto.
+  - unfold eq_dec. destruct EqDec_eq_of_X; auto.
+Qed.
+
+
+Lemma close_ld_type_notin : forall X e,
+    X `notin` ftv_in_dtyp (close_dtyp_wrt_dtyp X e).
+Proof.
+  intros. apply close_dtyp_notin_rec.
+Qed.
+
+Lemma d_subst_stv_in_dtyp_open_dtyp_wrt_dtyp_rec_mutual :
+(forall T3 T1 T2 SX n1,
+  lc_dtyp T1 ->
+  d_subst_stv_in_dtyp T1 SX (open_dtyp_wrt_dtyp_rec n1 T2 T3) = open_dtyp_wrt_dtyp_rec n1 (d_subst_stv_in_dtyp T1 SX T2) (d_subst_stv_in_dtyp T1 SX T3)).
+Proof.
+  apply_mutual_ind dtyp_mutind;
+  default_simp.
+  rewrite open_dtyp_wrt_dtyp_rec_degree_dtyp_wrt_dtyp; auto.
+  apply degree_dtyp_wrt_dtyp_O.
+  apply degree_dtyp_wrt_dtyp_of_lc_dtyp. auto.
+Qed.
+
+
+Lemma d_subst_stv_in_dtyp_open_dtyp_wrt_dtyp:
+forall T3 T1 T2 SX,
+  lc_dtyp T1 ->
+  d_subst_stv_in_dtyp T1 SX (open_dtyp_wrt_dtyp T3 T2) = open_dtyp_wrt_dtyp (d_subst_stv_in_dtyp T1 SX T3) (d_subst_stv_in_dtyp T1 SX T2).
+Proof.
+  unfold open_dtyp_wrt_dtyp; default_simp.
+  apply d_subst_stv_in_dtyp_open_dtyp_wrt_dtyp_rec_mutual. 
+  auto.
+Qed.
+
+Lemma d_subst_stv_in_dtyp_fresh_eq :
+(forall T2 T1 SX,
+  SX `notin` fstv_in_dtyp T2 ->
+  d_subst_stv_in_dtyp T1 SX T2 = T2).
+Proof.
+  apply_mutual_ind dtyp_mutind;
+  default_simp.
+Qed.
+
+Lemma d_subst_stv_in_dtyp_open_comm : forall SX T3 T1 T2,
+  lc_dtyp T3 -> 
+  SX `notin` fstv_in_dtyp T2 -> 
+  ({T3 /ₛᵈ SX} T1) ^^ᵈ T2 = {T3 /ₛᵈ SX} T1 ^^ᵈ T2.
+Proof.
+  intros.
+  rewrite d_subst_stv_in_dtyp_open_dtyp_wrt_dtyp.
+  rewrite (d_subst_stv_in_dtyp_fresh_eq T2); auto.
+  auto.
+Qed.
+
+
+Lemma dsubst_stv_lc_dtyp : forall SX T1 T2,
+  lc_dtyp T1 ->
+  lc_dtyp T2 ->
+  lc_dtyp ({ T2 /ₛᵈ SX } T1).
+Proof.
+  intros. induction H; simpl; auto.
+  - destruct (SX0 == SX); auto.
+  - eapply lc_dtyp_all. intros.
+    replace (({T2 /ₛᵈ SX} T) ^ᵈ X) with ({T2 /ₛᵈ SX} T ^ᵈ X); auto. 
+    rewrite d_subst_stv_in_dtyp_open_comm; auto.
+Qed.
+
+
+Hint Constructors ds_in_s: core.
+Hint Constructors ds_in: core.
+
+Lemma ftv_sin_dtyp_stvar_fstv_sin_dtyp : forall X T,
+  ds_in X T ->
+  ds_in_s X ({dtyp_svar X /ᵈ X} T).
+Proof.
+  intros. induction H; simpl; auto.
+  - destruct (X == X).
+    + constructor.
+    + contradiction.
+  - apply dsins_arrow1; auto.
+    now apply d_subst_tv_in_dtyp_lc_dtyp.
+  - apply dsins_arrow2; auto.
+    now apply d_subst_tv_in_dtyp_lc_dtyp.
+  - apply dsins_all with (L:=L `union` singleton X). intros.
+    inst_cofinites_with Y. 
+    replace (({dtyp_svar X /ᵈ X} T) ^ᵈ Y) with ({dtyp_svar X /ᵈ X} T ^ᵈ Y).
+    auto.
+    rewrite dtyp_subst_open_comm; auto.
+Qed.
+
+Lemma sin_in : forall X T, 
+  ds_in X T ->
+  X `in` ftv_in_dtyp T.
+Proof.
+  intros. induction H; simpl; auto.
+  - inst_cofinites_by (L `union` singleton X).
+    rewrite ftv_in_dtyp_open_dtyp_wrt_dtyp_upper in H0.
+    apply AtomSetImpl.union_1 in H0; inversion H0; auto.
+    + simpl in H1. apply AtomSetImpl.singleton_1 in H1.
+      apply notin_union_2 in Fr. subst.
+      apply notin_singleton_1 in Fr. contradiction.
+Qed.
+
+Lemma lc_dtyp_subst : forall T X S,
+  lc_dtyp ({S /ᵈ X} T) ->
+  lc_dtyp S ->
+  lc_dtyp T.
+Proof.
+  intros.
+  dependent induction H; auto.
+  - destruct T; try solve [inversion x]; auto.
+  - destruct T; try solve [inversion x]; auto.
+  - destruct T; try solve [inversion x]; auto.
+  - destruct T; try solve [inversion x]; auto.
+  - destruct T; try solve [inversion x]; auto.
+  - destruct T; try solve [inversion x]; auto.
+    inversion x; eauto.
+  - destruct T; try solve [inversion x]; auto.
+    inversion x. 
+    inst_cofinites_by (singleton X).
+    eapply lc_dtyp_all_exists with (X1:=x0). intros.
+    specialize (H0 x0 (T ^ᵈ x0) X S). apply H0.
+    subst. rewrite <- dtyp_subst_open_comm; auto.
+    auto.
+  - destruct T; try solve [inversion x]; auto.
+    inversion x; eauto.
+  - destruct T; try solve [inversion x]; auto.
+    inversion x; eauto.
+Qed.
+
+Lemma ftv_sin_dtyp_subst : forall X Y T S,
+  lc_dtyp S ->
+  X `notin` ftv_in_dtyp S ->
+  X <> Y ->
+  ds_in X ({S /ᵈ Y} T) ->
+  ds_in X T.
+Proof.
+  intros. dependent induction H2; simpl; auto.
+  - destruct T; simpl; try solve [inversion x].
+    inversion x. destruct (X0 == Y).
+    + subst. simpl in *. 
+      apply notin_singleton_1 in H0. contradiction.
+    + inversion H3. auto.
+  - destruct T; simpl; try solve [inversion x].
+    simpl in *. destruct (X0 == Y); subst.
+    + dependent destruction H.
+      simpl in H0.
+      eapply IHds_in with (S:=T1) (Y:=Y); auto. 
+      simpl. unfold eq_dec. destruct (EqDec_eq_of_X Y Y); auto.
+      contradiction. 
+    + inversion x.
+    + apply dsin_arrow1; inversion x; eauto.
+      subst.
+      eapply lc_dtyp_subst; eauto.
+  - destruct T; simpl; try solve [inversion x].
+    simpl in *. destruct (X0 == Y); subst.
+    + dependent destruction H.
+      simpl in H0. eapply IHds_in with (S:=T2) (Y:=Y); auto.
+      simpl. unfold eq_dec. destruct (EqDec_eq_of_X Y Y); auto.
+      contradiction. 
+    + inversion x.
+    + apply dsin_arrow2; inversion x; eauto.
+      subst. eapply lc_dtyp_subst; eauto.
+  - destruct T; simpl; try solve [inversion x].
+  simpl in *. destruct (X0 == Y); subst.
+    + assert (ds_in X (dtyp_all T0)).
+      * eapply dsin_all with (L:=L). intros. inst_cofinites_with Y0.
+        auto.
+      * apply sin_in in H4. contradiction.
+    + inversion x.
+    + apply dsin_all with (L:=L `union` singleton Y); intros; inst_cofinites_with Y0. auto.
+     inversion x. rewrite H6 in H3. 
+    eapply H2; eauto. subst. rewrite dtyp_subst_open_comm; auto.
+  - destruct T; simpl; try solve [inversion x].
+  simpl in *. destruct (X0 == Y); subst.
+    + assert (ds_in X (dtyp_union T1 T2)) by auto.
+      apply sin_in in H2. contradiction.
+    + inversion x.
+    + inversion x. apply dsin_union.
+      * eapply IHds_in1 with (S:=S) (Y:=Y); eauto.
+      * eapply IHds_in2 with (S:=S) (Y:=Y); eauto.
+  - destruct T; simpl; try solve [inversion x].
+    simpl in *. destruct (X0 == Y); subst.
+    + assert (ds_in X (dtyp_intersection T1 T2)) by auto.
+      apply sin_in in H2. contradiction.
+    + inversion x.
+    + inversion x. apply dsin_intersection.
+      * eapply IHds_in1 with (S:=S) (Y:=Y); eauto.
+      * eapply IHds_in2 with (S:=S) (Y:=Y); eauto.
+Qed.
+
+Lemma fstv_sin_dtyp_subst_tv : forall SX X T T',
+  ds_in_s SX T ->
+  lc_dtyp T' ->
+  ds_in_s SX ({T' /ᵈ X} T).
+Proof.
+  intros.
+  induction H; simpl; auto.
+  - apply dsins_arrow1; auto.
+    now apply d_subst_tv_in_dtyp_lc_dtyp.
+  - apply dsins_arrow2; auto.
+    now apply d_subst_tv_in_dtyp_lc_dtyp.
+  - simpl in H. 
+    apply dsins_all with (L:=L `union` singleton X). intros.
+    rewrite dtyp_subst_open_comm; auto.
+Qed.
+
+
+Lemma ftv_sins_dtyp_tvar_fstv_sin_dtyp : forall SX T,
+  ds_in_s SX T ->
+  ds_in SX ({dtyp_var_f SX /ₛᵈ SX} T).
+Proof.
+  intros. induction H; simpl; auto.
+  - destruct (SX == SX).
+    + constructor.
+    + contradiction.
+  - apply dsin_arrow1; auto.
+    apply dsubst_stv_lc_dtyp; auto.
+  - apply dsin_arrow2; auto.
+    apply dsubst_stv_lc_dtyp; auto.
+  - apply dsin_all with (L:=L `union` singleton SX). intros.
+    inst_cofinites_with Y. 
+    replace (({dtyp_var_f SX /ₛᵈ SX} T) ^ᵈ Y) with ({dtyp_var_f SX /ₛᵈ SX} T ^ᵈ Y).
+    auto.
+    rewrite d_subst_stv_in_dtyp_open_comm; auto.
+Qed.
+
+Lemma fstv_sins_dtyp_subst_stv : forall SX X T T',
+  ds_in X T ->
+  lc_dtyp T' ->
+  ds_in X ({T' /ₛᵈ SX} T).
+Proof.
+  intros.
+  induction H; simpl; auto.
+  - apply dsin_arrow1; auto.
+    now apply dsubst_stv_lc_dtyp.
+  - apply dsin_arrow2; auto.
+    now apply dsubst_stv_lc_dtyp.
+  - simpl in H. 
+    apply dsin_all with (L:=L `union` singleton X). intros.
+    rewrite d_subst_stv_in_dtyp_open_comm; auto.
+Qed.
+
+Lemma fstv_open_tvar : forall T SX,
+  SX `notin` fstv_in_dtyp T ->
+  ds_in_s SX (T ^^ᵈ dtyp_svar SX) ->
+  ds_in SX (T ^ᵈ SX).
+Proof.
+  intros.
+  replace (T ^ᵈ SX) with ({dtyp_var_f SX /ₛᵈ SX} T ^^ᵈ dtyp_svar SX).
+  apply ftv_sins_dtyp_tvar_fstv_sin_dtyp; auto.
+  rewrite d_subst_stv_in_dtyp_open_dtyp_wrt_dtyp; auto.
+  rewrite d_subst_stv_in_dtyp_fresh_eq; auto.
+  simpl. unfold eq_dec. destruct (EqDec_eq_of_X SX SX ); auto.
+  - contradiction.
+Qed.
+
+Lemma ftv_sin_dtyp_subst_inv : forall X Y T S,
+  lc_dtyp S ->
+  X <> Y ->
+  ds_in X T -> 
+  ds_in X ({S /ᵈ Y} T).
+Proof.
+  intros.
+  induction H1; try solve [simpl; eauto].
+  - simpl. destruct (X == Y).
+    + subst. contradiction.
+    + auto.
+  - simpl. apply dsin_arrow1; auto.
+    apply d_subst_tv_in_dtyp_lc_dtyp; auto.
+  - simpl. apply dsin_arrow2; auto.
+    apply d_subst_tv_in_dtyp_lc_dtyp; auto.
+  - simpl. eapply dsin_all with (L:=L `union` singleton Y).
+    intros. inst_cofinites_with Y0.
+    rewrite dtyp_subst_open_comm; auto.
+Qed.
+
+Lemma d_mono_typ_lc : forall T, 
+  dmono_typ T -> lc_dtyp T.
+Proof.
+  intros; induction H; auto.
+Qed.
+
+
+  
 
 (* Lemma ftv_in_dtyp_stvar_fstv_in_dtyp : forall X T,
   X `in` ftv_in_dtyp T ->
@@ -121,7 +468,7 @@ Qed. *)
 
 Lemma d_wf_typ_subst_tvar_stvar : forall E F X T,
   E ++ [(X, dbind_tvar_empty)] ++ F  ⊢ₛ T  -> 
-  map (dsubst_tv_in_binding (dtyp_svar X) X ) E ++ [(X, dbind_stvar_empty)] ++ F ⊢ₛ { dtyp_svar X /ᵈ X } T.
+  map (d_subst_tv_in_binding (dtyp_svar X) X ) E ++ [(X, dbind_stvar_empty)] ++ F ⊢ₛ { dtyp_svar X /ᵈ X } T.
 Proof.
   intros E F X T H.
   dependent induction H; try solve [simpl; auto].
@@ -148,17 +495,17 @@ Proof.
     + apply IHdwf_typ_s2; auto.
   - simpl. eapply dwftyps_all with (L:=L);
     intros; inst_cofinites_with SX.
-    + replace  (({dtyp_svar X /ᵈ X} T) ^^ᵈ dtyp_svar SX) with ({dtyp_svar X /ᵈ X} T ^^ᵈ dtyp_svar SX).
+    + replace  (({dtyp_svar X /ᵈ X} T1) ^^ᵈ dtyp_svar SX) with ({dtyp_svar X /ᵈ X} T1 ^^ᵈ dtyp_svar SX).
     apply fstv_sin_dtyp_subst_tv. auto.
     auto.
     rewrite dtyp_subst_open_comm; auto.
     + replace (SX ~ dbind_stvar_empty ++
-    map (dsubst_tv_in_binding (dtyp_svar X) X) E ++ (X, dbind_stvar_empty) :: F
+    map (d_subst_tv_in_binding (dtyp_svar X) X) E ++ (X, dbind_stvar_empty) :: F
     ) with (
-    map (dsubst_tv_in_binding (dtyp_svar X) X) (SX ~ dbind_stvar_empty ++ E) ++ (X, dbind_stvar_empty) :: F
+    map (d_subst_tv_in_binding (dtyp_svar X) X) (SX ~ dbind_stvar_empty ++ E) ++ (X, dbind_stvar_empty) :: F
     ) by auto.
-    replace (({dtyp_svar X /ᵈ X} T) ^^ᵈ dtyp_svar SX) with 
-    ({dtyp_svar X /ᵈ X} T ^^ᵈ dtyp_svar SX).
+    replace (({dtyp_svar X /ᵈ X} T1) ^^ᵈ dtyp_svar SX) with 
+    ({dtyp_svar X /ᵈ X} T1 ^^ᵈ dtyp_svar SX).
     apply H1. auto. 
     rewrite dtyp_subst_open_comm; auto. 
   - simpl. constructor.
@@ -172,7 +519,7 @@ Qed.
 
 Lemma d_wf_typ_subst_stvar_tvar : forall E F SX T,
   E ++ [(SX, dbind_stvar_empty)] ++ F  ⊢ T  -> 
-  map (dsubst_stv_in_binding (dtyp_var_f SX) SX ) E ++ [(SX, dbind_tvar_empty)] ++ F ⊢ { dtyp_var_f SX /ₛᵈ SX } T.
+  map (d_subst_stv_in_binding (dtyp_var_f SX) SX ) E ++ [(SX, dbind_tvar_empty)] ++ F ⊢ { dtyp_var_f SX /ₛᵈ SX } T.
 Proof.
   intros E F SX T H.
   dependent induction H; try solve [simpl; auto].
@@ -201,13 +548,13 @@ Proof.
     intros; inst_cofinites_with X.
     + replace  (({`ᵈ SX /ₛᵈ SX} T) ^ᵈ X) with ({`ᵈ SX /ₛᵈ SX} T ^ᵈ X).
       apply fstv_sins_dtyp_subst_stv; auto.
-      rewrite dsubst_stv_in_dtyp_open_comm; auto.
+      rewrite d_subst_stv_in_dtyp_open_comm; auto.
     + replace (X ~ dbind_tvar_empty ++
-    map (dsubst_stv_in_binding `ᵈ SX SX) E ++ (SX, dbind_tvar_empty) :: F) with (
-    map (dsubst_stv_in_binding `ᵈ SX SX) (X ~ dbind_tvar_empty ++ E) ++ (SX, dbind_tvar_empty) :: F) by auto.
+    map (d_subst_stv_in_binding `ᵈ SX SX) E ++ (SX, dbind_tvar_empty) :: F) with (
+    map (d_subst_stv_in_binding `ᵈ SX SX) (X ~ dbind_tvar_empty ++ E) ++ (SX, dbind_tvar_empty) :: F) by auto.
       replace (({`ᵈ SX /ₛᵈ SX} T) ^ᵈ X) with ({`ᵈ SX /ₛᵈ SX} T ^ᵈ X).
       apply H1. auto. 
-      rewrite dsubst_stv_in_dtyp_open_comm; auto.
+      rewrite d_subst_stv_in_dtyp_open_comm; auto.
   - simpl. constructor.
     + apply IHdwf_typ1; auto.
     + apply IHdwf_typ2; auto.
@@ -225,10 +572,10 @@ Proof.
   replace (X ~ dbind_tvar_empty ++ E) with (nil ++ X ~ dbind_tvar_empty ++ E) in H0 by auto.
   specialize (d_wf_typ_subst_tvar_stvar _ _ _ _ H0).
   intros.
-  rewrite dsubst_tv_in_dtyp_open_dtyp_wrt_dtyp in H1.
+  rewrite d_subst_tv_in_dtyp_open_dtyp_wrt_dtyp in H1.
   simpl in H1.
   unfold eq_dec in H1. destruct (EqDec_eq_of_X X X).
-  - rewrite dsubst_tv_in_dtyp_fresh_eq in H1; auto.
+  - rewrite d_subst_tv_in_dtyp_fresh_eq in H1; auto.
   - contradiction.
   - auto.
 Qed.
@@ -241,8 +588,8 @@ Proof.
   intros.
   replace (SX ~ dbind_stvar_empty ++ E) with (nil ++ SX ~ dbind_stvar_empty ++ E) in H0 by auto.
   specialize (d_wf_typ_subst_stvar_tvar _ _ _ _ H0). intros. 
-  rewrite dsubst_stv_in_dtyp_open_dtyp_wrt_dtyp in H1; auto. simpl in H1. unfold eq_dec in H1. destruct (EqDec_eq_of_X SX SX).
-  - rewrite dsubst_stv_in_dtyp_fresh_eq in H1; auto.
+  rewrite d_subst_stv_in_dtyp_open_dtyp_wrt_dtyp in H1; auto. simpl in H1. unfold eq_dec in H1. destruct (EqDec_eq_of_X SX SX).
+  - rewrite d_subst_stv_in_dtyp_fresh_eq in H1; auto.
   - contradiction.
 Qed.
 
@@ -255,9 +602,9 @@ Proof.
     intros; inst_cofinites_with SX.  
     + replace (T ^^ᵈ dtyp_svar SX) with ({dtyp_svar SX /ᵈ SX}T ^ᵈ SX).
       now apply ftv_sin_dtyp_stvar_fstv_sin_dtyp.
-      rewrite dsubst_tv_in_dtyp_open_dtyp_wrt_dtyp; auto.
+      rewrite d_subst_tv_in_dtyp_open_dtyp_wrt_dtyp; auto.
       simpl. unfold eq_dec. destruct (EqDec_eq_of_X SX SX).
-      * rewrite dsubst_tv_in_dtyp_fresh_eq; auto.
+      * rewrite d_subst_tv_in_dtyp_fresh_eq; auto.
       * contradiction.
     + apply d_wf_typ_subst_stvar_tvar_cons; auto.  
 Qed.
@@ -266,13 +613,13 @@ Lemma dwf_typ_s_dwf_typ : forall E T,
   E ⊢ₛ T -> E ⊢ T.
 Proof.
   intros. induction H; auto.
-  - eapply dwftyp_all with (L:= (L `union` fstv_in_dtyp T)); 
+  - eapply dwftyp_all with (L:= (L `union` fstv_in_dtyp T1)); 
     intros; inst_cofinites_with X.  
     + eapply fstv_open_tvar; auto. 
     + eapply d_wf_typ_subst_tvar_stvar_cons; auto.
 Qed.
 
-Hint Constructors dsub : core.
+Hint Constructors d_sub : core.
 Hint Resolve dwf_typ_dwf_typ_s : core.
 Hint Resolve dwf_typ_s_dwf_typ : core.
 
@@ -395,19 +742,19 @@ Lemma dwft_subst : forall E X T1 T2,
   E ⊢ T1 ^^ᵈ T2.
 Admitted.
 
-Hint Constructors dtyping : core.
+Hint Constructors d_typing : core.
 
 Lemma d_wft_typ_subst : forall E X F T1 T2,
   F ++ X ~ dbind_tvar_empty ++ E ⊢ T1 ->
   E ⊢ T2 ->
-  map (dsubst_tv_in_binding T2 X) F  ++ E ⊢ {T2 /ᵈ X} T1.
+  map (d_subst_tv_in_binding T2 X) F  ++ E ⊢ {T2 /ᵈ X} T1.
 Proof.
 Admitted.
 
 Lemma d_wf_env_subst_tvar_typ : forall E X F T1,
   ⊢ F ++ X ~ dbind_tvar_empty ++ E ->
   E ⊢ T1 ->
-  ⊢ (map (dsubst_tv_in_binding T1 X) F ++ E).
+  ⊢ (map (d_subst_tv_in_binding T1 X) F ++ E).
 Proof.
 Admitted.
 
@@ -433,6 +780,32 @@ Proof.
   intros. induction H; eauto.
 Qed.
 
+Hint Resolve d_mono_typ_lc : core.
+
+Lemma d_mono_typ_neq_all : forall T, 
+  dmono_typ T -> dneq_all T.
+Proof.
+  intros; induction H; auto...
+Qed.
+
+Lemma d_neq_all_subst_neq_all : forall T1 X T2,
+  lc_dtyp T1 ->
+  dmono_typ T2 ->
+  dneq_all T1 ->
+  dneq_all ( {T2 /ᵈ X} T1 ).
+Proof.
+  intros. induction H; simpl; eauto...
+  - destruct (X0 == X); auto.
+    apply d_mono_typ_neq_all; auto. 
+  - eapply dneqall_arrow; 
+    apply d_subst_tv_in_dtyp_lc_dtyp; eauto...
+  - inversion H1.
+  - eapply dneqall_union; 
+    apply d_subst_tv_in_dtyp_lc_dtyp; eauto...
+  - eapply dneqall_intersection; 
+    apply d_subst_tv_in_dtyp_lc_dtyp; eauto...
+Qed.
+
 Lemma wft_all_open_wfdtyp_wft : forall E X T1 T2,
   E ⊢ T1 ->
   E ⊢ T2 ->
@@ -456,13 +829,13 @@ Lemma bind_typ_subst : forall F X E x T1 T2,
   ⊢ F ++ (X, dbind_tvar_empty) :: E ->
   binds x (dbind_typ T1) (F ++ (X, dbind_tvar_empty) :: E) ->
   E ⊢ T2 ->
-  binds x (dbind_typ ({T2 /ᵈ X} T1)) (map (dsubst_tv_in_binding T2 X) F ++ E).
+  binds x (dbind_typ ({T2 /ᵈ X} T1)) (map (d_subst_tv_in_binding T2 X) F ++ E).
 Proof.
   intros. induction F; simpl in *; auto.
   - inversion H0.
     + inversion H2.
     + assert (E ⊢ T1) by admit.
-      rewrite dsubst_tv_in_dtyp_fresh_eq; auto.
+      rewrite d_subst_tv_in_dtyp_fresh_eq; auto.
       eapply d_new_tv_notin_wf_typ; eauto.
   - destruct a. inversion H0.
     + inversion H2. auto.
@@ -490,21 +863,21 @@ Lemma dsub_dwft : forall E T1 T2,
 Proof.
   intros.
   induction H; try solve [intuition].
-  - split; eapply dwftyp_all with (L:=L `union` fstv_in_dtyp S `union` fstv_in_dtyp T); intros; inst_cofinites_with X.
+  - split; eapply dwftyp_all with (L:=L `union` fstv_in_dtyp S1 `union` fstv_in_dtyp T1); intros; inst_cofinites_with X.
     + eapply fstv_open_tvar; auto.
     + apply d_wf_typ_subst_tvar_stvar_cons; intuition.
     + eapply fstv_open_tvar; auto.
     + apply d_wf_typ_subst_tvar_stvar_cons; intuition.
   - split; try solve [intuition].
-    + eapply dwftyp_all with (L:=L `union` ftv_in_dtyp S). 
+    + eapply dwftyp_all with (L:=L `union` ftv_in_dtyp S1). 
       * intros. inst_cofinites_with X. auto.
       * intros. inst_cofinites_with X.
-        destruct IHdsub. 
+        destruct IHd_sub. 
         eapply dwf_typ_open_inv with (X:=X) (S:=T2); auto.
-        eapply dwf_typ_dlc_type; eauto.
-        -- replace (X ~ dbind_tvar_empty ++ E) with (nil ++ X ~ dbind_tvar_empty ++ E) by auto. apply dwf_typ_weakening. simpl. rewrite  dsubst_tv_in_dtyp_open_dtyp_wrt_dtyp.
-          ++ simpl. unfold eq_dec. destruct ( EqDec_eq_of_X X X ).
-            ** rewrite dsubst_tv_in_dtyp_fresh_eq; auto.
-            ** contradiction.
-          ++ eapply dwf_typ_dlc_type; eauto.
+        -- replace (X ~ dbind_tvar_empty ++ E) with (nil ++ X ~ dbind_tvar_empty ++ E) by auto. 
+           apply dwf_typ_weakening. simpl. rewrite  d_subst_tv_in_dtyp_open_dtyp_wrt_dtyp.
+           ++ simpl. unfold eq_dec. destruct ( EqDec_eq_of_X X X ).
+              ** rewrite d_subst_tv_in_dtyp_fresh_eq; auto.
+              ** contradiction.
+           ++ eapply dwf_typ_dlc_type; eauto.
 Qed.
