proof/iu_system/decl/prop_type_safety.v
@@ -29,7 +29,7 @@ Inductive empty_var_dom : denv -> Prop :=
 
 
 (* Lemma canonical_form_abs : forall E e m,
-  dtyping E e m dtyp_bot -> 
+  d_typing E e m dtyp_bot -> 
   var_dom E = empty ->
   is_dvalue_of_dexp e = true ->
   False.
@@ -59,7 +59,7 @@ Proof.
 Qed.
 
 Theorem typing_all_inversion : forall E e T,
-  dtyping E e dtypingmode_inf (dtyp_all T) ->
+  d_typing E e d_typingmode_inf (dtyp_all T) ->
   empty_var_dom E ->
   d_isval e ->
   (exists e1 T1, e = dexp_tabs (dbody_anno e1 T1)) \/ (exists e1 T1, e = dexp_anno (dexp_abs e1) (dtyp_all T1)).
@@ -76,8 +76,8 @@ Qed.
   end.
 
 Theorem typing_all_inversion3 : forall E e m T,
-  dtyping E e m (dtyp_all T) ->
-  m = dtypingmode_chk \/ m = dtypingmode_inf ->
+  d_typing E e m (dtyp_all T) ->
+  m = d_typingmode_chk \/ m = d_typingmode_inf ->
   empty_var_dom E ->
   is_dvalue_of_dexp e = true ->
   (exists e1 T1, e = dexp_tabs (dbody_anno e1 T1)) \/ (exists e1 T1, e = dexp_anno (dexp_tabs (dbody_anno e1 T1)) (dtyp_all T)).
@@ -86,10 +86,10 @@ Proof.
   dependent induction H; try solve [inversion H3]; 
   try solve [inversion H1].
   - assert 
-    (dtypingmode_chk = dtypingmode_chk ∨ dtypingmode_chk = dtypingmode_inf) by auto. 
+    (d_typingmode_chk = d_typingmode_chk ∨ d_typingmode_chk = d_typingmode_inf) by auto. 
     simpl in H3.
-    specialize (IHdtyping T (eq_refl _) H4 H2 H3).
-    inversion IHdtyping.
+    specialize (IHd_typing T (eq_refl _) H4 H2 H3).
+    inversion IHd_typing.
     + destruct H5 as [e1 [T1]]. right.
       rewrite H5. eauto.
     + admit. (* should allow n'fold anno, exists n e1 t1, e = dexp_anno^n ((dexp_tabs (dbody_anno e1 T1))) *)
@@ -105,9 +105,9 @@ Admitted.
 
 
  Theorem typing_all_inversion5 : forall E e m S T,
-  dtyping E e m S ->
+  d_typing E e m S ->
   dsub E S (dtyp_all T) ->
-  m = dtypingmode_chk \/ m = dtypingmode_inf ->
+  m = d_typingmode_chk \/ m = d_typingmode_inf ->
   empty_var_dom E ->
   is_dvalue_of_dexp e = true ->
   (exists e1 T1, e = dexp_tabs (dbody_anno e1 T1)) \/ (exists e1 T1, e = dexp_anno (dexp_tabs (dbody_anno e1 T1)) (dtyp_all T)).
@@ -116,10 +116,10 @@ Proof.
   generalize dependent T.
   dependent induction Htyping; intros T0 Hsub; try solve [inversion Heqv]; try solve [inversion Hsub].
   (* - assert 
-  (dtypingmode_chk = dtypingmode_chk ∨ dtypingmode_chk = dtypingmode_inf) by auto. 
+  (d_typingmode_chk = d_typingmode_chk ∨ d_typingmode_chk = d_typingmode_inf) by auto. 
   simpl in H3.
-  specialize (IHdtyping T (eq_refl _) H4 H2 H3).
-  inversion IHdtyping.
+  specialize (IHd_typing T (eq_refl _) H4 H2 H3).
+  inversion IHd_typing.
   + destruct H5 as [e1 [T1]]. right.
     rewrite H5. eauto.
   + admit. should allow n'fold anno, exists n e1 t1, e = dexp_anno^n ((dexp_tabs (dbody_anno e1 T1))) *)
@@ -141,9 +141,9 @@ Admitted.
 
 
 Theorem typing_all_inversion6 : forall E e m S T L,
-  dtyping E e m S ->
+  d_typing E e m S ->
   (forall X, X `notin` L -> dsub E S (open_dtyp_wrt_dtyp T (dtyp_var_f X))) ->
-  m = dtypingmode_chk \/ m = dtypingmode_inf ->
+  m = d_typingmode_chk \/ m = d_typingmode_inf ->
   empty_var_dom E ->
   is_dvalue_of_dexp e = true ->
   (exists e1 T1 n, e = anno_nfold n e1 T1 T).
@@ -154,36 +154,36 @@ generalize dependent L.
 (* generalize dependent X. *)
 dependent induction Htyping; intros L0 T0 Hsub; try solve [inversion Heqv]; try solve [inversion Hsub].
 (* - assert 
-(dtypingmode_chk = dtypingmode_chk ∨ dtypingmode_chk = dtypingmode_inf) by auto. 
+(d_typingmode_chk = d_typingmode_chk ∨ d_typingmode_chk = d_typingmode_inf) by auto. 
 simpl in H3.
-specialize (IHdtyping T (eq_refl _) H4 H2 H3).
-inversion IHdtyping.
+specialize (IHd_typing T (eq_refl _) H4 H2 H3).
+inversion IHd_typing.
 + destruct H5 as [e1 [T1]]. right.
   rewrite H5. eauto.
 + admit. should allow n'fold anno, exists n e1 t1, e = dexp_anno^n ((dexp_tabs (dbody_anno e1 T1))) *)
-- assert (dtypingmode_chk = dtypingmode_chk ∨ dtypingmode_chk = dtypingmode_inf) by auto.
+- assert (d_typingmode_chk = d_typingmode_chk ∨ d_typingmode_chk = d_typingmode_inf) by auto.
   specialize (IHHtyping H0 Hemp Heqv L0 T0 Hsub).
   admit.
 - admit. (* impossible *)
 - inst_cofinites_by L.
-assert (dtypingmode_chk = dtypingmode_chk ∨ dtypingmode_chk = dtypingmode_inf) by auto. admit.
+assert (d_typingmode_chk = d_typingmode_chk ∨ d_typingmode_chk = d_typingmode_inf) by auto. admit.
 - admit. (* impossible *)
 - admit. (* impossible *)
 Admitted. 
 
 Theorem typing_all_inversion4 : forall e m T,
-  dtyping nil e m (dtyp_all T) ->
-  m = dtypingmode_chk \/ m = dtypingmode_inf ->
+  d_typing nil e m (dtyp_all T) ->
+  m = d_typingmode_chk \/ m = d_typingmode_inf ->
   is_dvalue_of_dexp e = true ->
   (exists e1 T1, e = dexp_tabs (dbody_anno e1 T1)) \/ (exists e1 T1, e = dexp_anno (dexp_tabs (dbody_anno e1 T1)) (dtyp_all T)).
 Proof.
   intros.
   dependent induction H; try solve [inversion H2].
   - assert
-    (dtypingmode_chk = dtypingmode_chk ∨ dtypingmode_chk = dtypingmode_inf) by auto. 
+    (d_typingmode_chk = d_typingmode_chk ∨ d_typingmode_chk = d_typingmode_inf) by auto. 
     simpl in H2.
-    specialize (IHdtyping T (JMeq_refl _) (eq_refl _) H3 H2).
-    inversion IHdtyping.
+    specialize (IHd_typing T (JMeq_refl _) (eq_refl _) H3 H2).
+    inversion IHd_typing.
     + destruct H4 as [e1 [T1]]. right.
       rewrite H4. eauto.
     + admit. (* should allow n'fold anno, exists n e1 t1, e = dexp_anno^n ((dexp_tabs (dbody_anno e1 T1))) *)
@@ -199,19 +199,19 @@ Admitted.
 
 (* 
 Theorem progress1 : forall e m T,
-  dtyping nil e m T ->
+  d_typing nil e m T ->
   is_dvalue_of_dexp e = true \/ exists e', dexp_red e e'.
 Proof.
   intros. dependent induction H; intros; auto.
-  - specialize (IHdtyping (JMeq_refl _)).
-    inversion IHdtyping.
+  - specialize (IHd_typing (JMeq_refl _)).
+    inversion IHd_typing.
     + left. auto.
     + right. destruct H1 as [e']. eauto.
   (* e1 e2 *)
-  - specialize (IHdtyping1 (JMeq_refl _)). 
-    specialize (IHdtyping2 (JMeq_refl _)). 
-    inversion IHdtyping1.
-    + inversion IHdtyping2.
+  - specialize (IHd_typing1 (JMeq_refl _)). 
+    specialize (IHd_typing2 (JMeq_refl _)). 
+    inversion IHd_typing1.
+    + inversion IHd_typing2.
       * admit. (* medium : inversion lemma of app *)
       * destruct H2 as [e2']. right. exists (dexp_app e1 e2'). 
         apply dexpred_app2; auto. 
@@ -221,7 +221,7 @@ Proof.
       constructor; auto.
       admit. (* easy : lc *)
   (* e => BOT *)
-  - specialize (IHdtyping  (JMeq_refl _)). inversion IHdtyping.
+  - specialize (IHd_typing  (JMeq_refl _)). inversion IHd_typing.
     + destruct e; try solve [inversion H1; inversion H0].
       * dependent destruction H0. inversion H2.
         right. exists (dexp_anno e dtyp_bot).  constructor.
@@ -229,8 +229,8 @@ Proof.
         admit. admit. (* easy : lc *)
     + right. destruct H1 as [e']. eauto.
   (* e @ T *)
-  - specialize (IHdtyping  (JMeq_refl _)).
-    inversion IHdtyping.
+  - specialize (IHd_typing  (JMeq_refl _)).
+    inversion IHd_typing.
     + admit. (* medium : inversion lemma of tapp *)
     + right. destruct H1 as [e1']. eauto.
   (* e => ∀ X . T *)
@@ -239,21 +239,21 @@ Admitted. *) *)
 
 
 Theorem progress' : forall E e m T,
-  dtyping E e m T ->
+  d_typing E e m T ->
   empty_var_dom E ->
   d_isval e \/ exists e', dexp_red e e'.
 Proof.
   intros. dependent induction H; intros; auto.
   - exfalso; eapply bind_var_var_dom_not_empty; eauto.
-  - specialize (IHdtyping H1).
-    inversion IHdtyping.
+  - specialize (IHd_typing H1).
+    inversion IHd_typing.
     + admit.
     + right. destruct H2 as [e']. eauto.
   (* e1 e2 *)
-  - specialize (IHdtyping1 H1). 
-    specialize (IHdtyping2 H1). 
-    inversion IHdtyping1.
-    + inversion IHdtyping2.
+  - specialize (IHd_typing1 H1). 
+    specialize (IHd_typing2 H1). 
+    inversion IHd_typing1.
+    + inversion IHd_typing2.
       * dependent destruction H2.
         -- dependent destruction H. inversion H0.
         -- dependent destruction H.
@@ -268,7 +268,7 @@ Proof.
       admit. (* easy : lc *)
   - left; admit. (* easy : lc *)
   (* e => BOT *)
-  - specialize (IHdtyping H1). inversion IHdtyping.
+  - specialize (IHd_typing H1). inversion IHd_typing.
   
     + destruct e; try solve [inversion H2; inversion H0].
       * dependent destruction H0. dependent destruction H3.
@@ -277,8 +277,8 @@ Proof.
         admit. (* easy : lc *)
     + right. destruct H2 as [e']. eauto.
   (* e @ T *)
-  - specialize (IHdtyping H1).
-    inversion IHdtyping.
+  - specialize (IHd_typing H1).
+    inversion IHd_typing.
     + specialize (typing_all_inversion _ _ _ H0 H1 H2).
       intros. inversion H3.
       * destruct H4 as [e3 [T3]]. rewrite H4.
@@ -294,16 +294,16 @@ Admitted.
 
 
 Theorem progress : forall e m T,
-  dtyping nil e m T ->
+  d_typing nil e m T ->
   d_isval e \/ exists e', dexp_red e e'.
 Proof.
   intros. eapply progress'; eauto.
 Qed.
 
-Hint Constructors dtyping : type_safety.
+Hint Constructors d_typing : type_safety.
 
 Lemma check_top_false : forall E T,
-  dtyping E dexp_top dtypingmode_chk T -> E ⊢ dtyp_top <: T.
+  d_typing E dexp_top d_typingmode_chk T -> E ⊢ dtyp_top <: T.
 Proof.
   intros; dependent induction H; eauto...
   - inversion H. inst_cofinites_by (L `union` L0). 
@@ -312,7 +312,7 @@ Proof.
 Qed.
 
 Lemma check_unit_false : forall E T,
-  dtyping E dexp_unit dtypingmode_chk T -> E ⊢ dtyp_unit <: T.
+  d_typing E dexp_unit d_typingmode_chk T -> E ⊢ dtyp_unit <: T.
 Proof.
   intros; dependent induction H; eauto...
   - inversion H. inst_cofinites_by (L `union` L0). 
@@ -323,9 +323,9 @@ Qed.
 (* E |- e <= T 
 [t2 / x] E |- [t2 / x] e <= [t2 / x] T *)
 Theorem preservation : forall E e e' m T,
-  dtyping E e m T -> 
+  d_typing E e m T -> 
   dexp_red e e' -> 
-  dtyping E e' m T.
+  d_typing E e' m T.
 Proof with eauto with type_safety.
   intros. generalize dependent e'.
   induction H; intros e' Hred; try solve [inversion Hred]; eauto...
@@ -357,7 +357,7 @@ Proof with eauto with type_safety.
         admit.
         simpl. admit. 
       * inst_cofinites_by L. admit.
-    + dependent destruction H0. eapply dtyping_infanno.
+    + dependent destruction H0. eapply d_typing_infanno.
       admit. admit.
     + inversion H0.
 Admitted.
